Linearize: utilisation d'une heuristique externe d'enumeration des noeuds du CFG
git-svn-id: https://yquem.inria.fr/compcert/svn/compcert/trunk@437 fca1b0fc-160b-0410-b1d3-a4f43f01ea2e

caml/Linearizeaux.ml
@@ -1,0 +1,83 @@
+open BinPos
+open Coqlib
+open Datatypes
+open LTL
+open Lattice
+open CList
+open Maps
+open Camlcoq
+
+(* Trivial enumeration, in decreasing order of PC *)
+
+(***
+let enumerate_aux f reach =
+  positive_rec
+    Coq_nil
+    (fun pc nodes ->
+      if PMap.get pc reach
+      then Coq_cons (pc, nodes)
+      else nodes) 
+    f.fn_nextpc
+***)
+
+(* More clever enumeration that flattens basic blocks *)
+
+let rec int_of_pos = function
+  | Coq_xI p -> (int_of_pos p lsl 1) + 1
+  | Coq_xO p -> int_of_pos p lsl 1
+  | Coq_xH -> 1
+
+(* Count the reachable predecessors for each node *)
+
+let reachable_predecessors f reach =
+  let count = Array.make (int_of_pos f.fn_nextpc) 0 in
+  let increment pc =
+    let i = int_of_pos pc in
+    count.(i) <- count.(i) + 1 in
+  positive_rec
+    ()
+    (fun pc _ ->
+      if PMap.get pc reach then coqlist_iter increment (successors f pc))
+    f.fn_nextpc;
+  count
+
+(* Recognize instructions with only one successor *)
+
+let single_successor f pc =
+  match PTree.get pc f.fn_code with
+    | Some i ->
+        (match i with
+           | Lnop s -> Some s
+           | Lop (op, args, res, s) -> Some s
+           | Lload (chunk, addr, args, dst, s) -> Some s
+           | Lstore (chunk, addr, args, src, s) -> Some s
+           | Lcall (sig0, ros, args, res, s) -> Some s
+           | Ltailcall (sig0, ros, args) -> None
+           | Lalloc (arg, res, s) -> Some s
+           | Lcond (cond, args, ifso, ifnot) -> None
+           | Lreturn optarg -> None)
+    | None -> None
+
+(* Build the enumeration *)
+
+let enumerate_aux f reach =
+  let preds = reachable_predecessors f reach in
+  let enum = ref Coq_nil in
+  let emitted = Array.make (int_of_pos f.fn_nextpc) false in
+  let rec emit_basic_block pc =
+    enum := Coq_cons(pc, !enum);
+    emitted.(int_of_pos pc) <- true;
+    match single_successor f pc with
+    | None -> ()
+    | Some pc' ->
+        let npc' = int_of_pos pc' in
+        if preds.(npc') <= 1 && not emitted.(npc') then emit_basic_block pc' in
+  let rec emit_all pc =
+    if pc <> Coq_xH then begin
+      let pc = coq_Ppred pc in
+      if not emitted.(int_of_pos pc) && PMap.get pc reach
+      then emit_basic_block pc;
+      emit_all pc
+    end in
+  emit_all f.fn_nextpc;
+  CList.rev !enum
